Lean4Lean/Expr.lean
@@ -20,20 +20,6 @@ def realLooseBVarRange : Expr → Nat
   | .forallE _ e1 e2 _ => max e1.realLooseBVarRange (e2.realLooseBVarRange - 1)
   | .letE _ e1 e2 e3 _ => max (max e1.realLooseBVarRange e2.realLooseBVarRange) (e3.realLooseBVarRange - 1)
 
-def Safe : Expr → Prop
-  | .bvar i => i < 2^20 - 1
-  | .const ..
-  | .sort _ -- TODO: should this use Level.Safe?
-  | .fvar _
-  | .mvar _
-  | .lit _ => True
-  | .mdata _ e
-  | .proj _ _ e => e.Safe
-  | .app e1 e2
-  | .lam _ e1 e2 _
-  | .forallE _ e1 e2 _ => e1.Safe ∧ e2.Safe
-  | .letE _ e1 e2 e3 _ => e1.Safe ∧ e2.Safe ∧ e3.Safe
-
 namespace ReplaceImpl
 
 unsafe abbrev ReplaceT := StateT (PtrMap Expr Expr)
